plugin/theories/Egg.v
@@ -1,2 +1,32 @@
-Definition trigger{A: Type}(a: A) := True.
-Register trigger as egg.trigger.
+Inductive dyn_list: Type :=
+| dyn_nil
+| dyn_cons{A: Type}(head: A)(tail: dyn_list).
+Register dyn_list as egg.dyn_list.
+Register dyn_nil as egg.dyn_nil.
+Register dyn_cons as egg.dyn_cons.
+
+Declare Custom Entry dyn_list.
+Notation "x" := (dyn_cons x dyn_nil)
+  (in custom dyn_list at level 0, x constr at level 0).
+Notation "h t" := (dyn_cons h t)
+  (in custom dyn_list at level 0, h constr at level 0, t custom dyn_list at level 0).
+
+Notation "'dyn_list:(' l ')'" := l
+  (l custom dyn_list at level 1, format "dyn_list:( l )").
+
+Goal dyn_list:(true) <> dyn_list:(1 (2 = 2) true). Abort.
+
+Definition with_trigger(t: dyn_list)(P: Prop) := P.
+Register with_trigger as egg.with_trigger.
+
+Notation "'trigger!' ( t ) P" := (with_trigger t P)
+  (at level 10, t custom dyn_list at level 0, P constr at level 0,
+   format "trigger!  ( t )  P").
+
+Goal (forall a b : nat, trigger! ((a * b)) (0 <= a -> 0 <= b -> 0 <= a * b))
+   = (forall a b: nat, with_trigger (dyn_cons (a * b) dyn_nil)
+                                    (0 <= a -> 0 <= b -> 0 <= a * b)).
+Proof. reflexivity. Abort.
+
+Goal (forall a b : nat, trigger! ((a * b) (b * a)) (0 <= a -> 0 <= b -> 0 <= a * b)).
+Abort.
